update

model.v
@@ -28,7 +28,7 @@ Section Histories.
                    | _, _ => false
     end.
   Inductive mode : Type :=
-  | Commute : mode
+  | ConflictFree : mode
   | Oracle : mode
   | Replay : mode.
 
@@ -86,12 +86,12 @@ Section MachineState.
   
   Record state := mkState { X_copy : history;
                             Y_copy : tid -> history;
-                            preH : history;
-                            commH : tid -> history;
-                            postH : history;
+                            X_performed : history;
+                            Y_performed : tid -> history;
+                            oracle_performed : history;
                             md : mode
                           }.
-  Definition start_mode := match X with | [] => Commute | _ => Replay end.
+  Definition start_mode := match X with | [] => ConflictFree | _ => Replay end.
   Definition start_state : state :=
     mkState X (history_of_thread Y) [] (fun tid => []) [] start_mode.
                                         
@@ -114,13 +114,13 @@ Section Machine.
   Definition combined_histories (histories : tid -> history) :=
     combine_tid_histories histories num_threads.
   Definition get_state_history (s : state) :=
-    s.(postH) ++ combined_histories s.(commH) ++ s.(preH).
+    s.(oracle_performed) ++ combined_histories s.(Y_performed) ++ s.(X_performed).
   Definition state_with_md (s : state) (md : mode) :=
-    mkState s.(X_copy) s.(Y_copy) s.(preH) s.(commH) s.(postH) md.
+    mkState s.(X_copy) s.(Y_copy) s.(X_performed) s.(Y_performed) s.(oracle_performed) md.
 
   Definition get_oracle_response (s : state) (t: tid) (i: invocation) : state * action :=
     let resp := oracle_response (get_state_history s) t i in
-    (mkState (s.(X_copy)) (s.(Y_copy)) (s.(preH)) (s.(commH)) ((t,i,resp)::s.(postH)) Oracle,
+    (mkState (s.(X_copy)) (s.(Y_copy)) (s.(X_performed)) (s.(Y_performed)) ((t,i,resp)::s.(oracle_performed)) Oracle,
      (t,i,resp)).
 
   Definition get_commute_response (s : state) (t: tid) (i: invocation) : state * action :=
@@ -128,24 +128,24 @@ Section Machine.
       | hd::tl => (mkState s.(X_copy)
                                (fun tid => if tid =? t then (rev tl)
                                            else s.(Y_copy) tid)
-                               s.(preH) (fun tid => if tid =? t then hd::(s.(commH) t)
-                                                    else s.(commH) tid)
-                                        s.(postH) Commute, hd)
+                               s.(X_performed) (fun tid => if tid =? t then hd::(s.(Y_performed) t)
+                                                    else s.(Y_performed) tid)
+                                        s.(oracle_performed) ConflictFree, hd)
       | _ => (s, (t,i,NoResp)) (* should never hit this *)
     end.
     
   Definition get_replay_response (s : state) (t: tid) (i : invocation) : state * action :=
     match rev s.(X_copy) with
-    | hd::tl => (mkState (rev tl) s.(Y_copy) (hd::s.(preH)) s.(commH) s.(postH) s.(md), hd)
-    | _ => (mkState s.(X_copy) s.(Y_copy) ((t,i,NoResp)::s.(preH)) s.(commH) s.(postH) s.(md),
+    | hd::tl => (mkState (rev tl) s.(Y_copy) (hd::s.(X_performed)) s.(Y_performed) s.(oracle_performed) s.(md), hd)
+    | _ => (mkState s.(X_copy) s.(Y_copy) ((t,i,NoResp)::s.(X_performed)) s.(Y_performed) s.(oracle_performed) s.(md),
            (t,i,NoResp)) (* should never hit this *)
     end.
   Definition next_mode (s : state) (t: tid) (i: invocation) : mode :=
     match s.(md) with
       | Oracle => Oracle
-      | Commute => match rev (s.(Y_copy) t) with
+      | ConflictFree => match rev (s.(Y_copy) t) with
                      | [] => Oracle
-                     | hd :: tl => if action_invocation_eq hd t i then Commute
+                     | hd :: tl => if action_invocation_eq hd t i then ConflictFree
                                    else Oracle
                    end
       | Replay => match rev s.(X_copy) with
@@ -158,10 +158,10 @@ Section Machine.
     let mode := next_mode s t i in
     match mode with
       | Oracle => get_oracle_response (state_with_md s Oracle) t i
-      | Commute => get_commute_response (state_with_md s Commute) t i
+      | ConflictFree => get_commute_response (state_with_md s ConflictFree) t i
       | Replay => match rev (s.(X_copy)) with
-                  | [hd] => get_replay_response (state_with_md s Commute) t i
-                                                (* Changes mode to Commute *)
+                  | [hd] => get_replay_response (state_with_md s ConflictFree) t i
+                                                (* Changes mode to ConflictFree *)
                   | _ => get_replay_response (state_with_md s Replay) t i
                   end
     end.
@@ -176,24 +176,24 @@ Section Machine.
 End Machine.
 
 Section Conflict.
-  Definition write_tid_set {A : Type} (ts1 ts2 : tid -> A) : Ensemble tid :=
+  Definition diff_histories_tid_set {A : Type} (ts1 ts2 : tid -> A) : Ensemble tid :=
     fun tid => ts1 tid <> ts2 tid.
-  Definition step_writes (s1 s2 : state) : Ensemble tid :=
+  Definition diff_states_tid_set (s1 s2 : state) : Ensemble tid :=
     Union tid
-          (write_tid_set s1.(commH) s2.(commH))
-          (write_tid_set s1.(Y_copy) s2.(Y_copy)).
+          (diff_histories_tid_set s1.(Y_performed) s2.(Y_performed))
+          (diff_histories_tid_set s1.(Y_copy) s2.(Y_copy)).
  Definition conflict_free_writes (t :tid) (s1 s2 : state) :=
-   step_writes s1 s2 = Singleton tid t /\
+   diff_states_tid_set s1 s2 = Singleton tid t /\
    s1.(md) = s2.(md) /\
    s1.(X_copy) = s2.(X_copy) /\
-   s1.(preH) = s2.(preH) /\
-   s1.(postH) = s2.(postH).
+   s1.(X_performed) = s2.(X_performed) /\
+   s1.(oracle_performed) = s2.(oracle_performed).
  Definition conflict_free_reads t i s :=
    forall (s1 s2 s1' s2': state) (a1 a2: action),
      s1.(Y_copy) t = s.(Y_copy) t ->
      s2.(Y_copy) t = s.(Y_copy) t ->
-     s1.(commH) t = s.(commH) t ->
-     s2.(commH) t = s.(commH) t ->
+     s1.(Y_performed) t = s.(Y_performed) t ->
+     s2.(Y_performed) t = s.(Y_performed) t ->
      s1.(md) = s.(md) ->
      s2.(md) = s.(md) ->
      machine_act s1 t i = (s1', a1) ->
